(Change of variables formula). Let $(X,\mathcal{B},\mu)$ be a measure space, and let $\phi:X\to Y$ be a measurable morphism (as defined in Remark 1.4.33) from $(X,\mathcal{B})$ to another measurable space $(Y,\mathcal{C})$. Define the pushforward $\phi _* \mu: \mathcal{C}\to [0,+\infty]$ of $\mu$ by $\phi$ by the formula $\phi _* \mu (E) \coloneqq \mu(\phi ^{-1}(E))$.
1. Show that $\phi _* \mu$ is a measure on $\mathcal{C}$, so that $(Y,\mathcal{C},\phi _* \mu)$ is a measure space.
2. If $f: Y\to [0,+\infty]$ is measurable, show that $\int _Y f\ d \phi _* \mu=\int _X (f\circ \phi)\ d\mu$.